test_databases/include_depth/level2_ok.mm
@@ -1,0 +1,3 @@
+$c wff $.
+$v x $.
+fx $f wff x $.
