test_databases/include_depth/root_depth.mm
@@ -1,0 +1,1 @@
+$[ level1_depth.mm $]
