test_databases/include_policy/inner_scope_violation.mm
@@ -1,0 +1,3 @@
+${ 
+$[ non_existent_include.mm $]
+$}
