test_databases/include_policy/inside_statement_violation.mm
@@ -1,0 +1,2 @@
+$c wff x $.
+ax-include $a wff x $[ non_existent_include.mm $] $.
