test_databases/include_policy/missing_include_read_failure.mm
@@ -1,0 +1,1 @@
+$[ definitely_missing_include_file_42.mm $]
